\documentclass[12pt]{article}
\usepackage[utf8]{inputenc}
\usepackage{amsmath}
\usepackage{graphicx}

\begin{document}

Esimene ülesanne

\begin{displaymath}
\dfrac{
	\dfrac{
		\dfrac{
		}{
			\{a:\alpha, x:\alpha\}\vdash \, x :\,\alpha
		}
	}{
		\{a:\alpha\}\vdash \, (\lambda x:\alpha. x) :\, \alpha\to\alpha
	} 
	\quad
	\dfrac{
	}{
		\{a:\alpha\}\vdash \, a:\,\alpha
	}
}{
	\{a : \alpha\} \vdash (\lambda x:\alpha. x)\, a :\, \alpha
}
\end{displaymath}

Teine ülesanne

\begin{displaymath}
\dfrac{
	\dfrac{
		\{x:\alpha\}\vdash x\,x:?
	}{
		\vdash (\lambda x:\alpha. x\,x)\,:?
	}
		\quad
		\dfrac{
			\dfrac{
				\dfrac{
				}{
					\{x:\alpha\}\vdash x:\,\alpha
				}
				\quad
				\dfrac{
				}{
					\{x:\alpha\}\vdash x:\,\alpha
				}
		}{
			\{x:\alpha\}\vdash x\,x:?}}{\vdash (\lambda x:\alpha. x\,x)\,:\,?
		}
}{
	\vdash (\lambda x:\alpha. x\,x)\,(\lambda x:\alpha. x\,x) :\,?
}
\end{displaymath}
Ei saa lahendada, aplikatsioon ei tule kujul $muutuja\to muutuja$

\\~\\

Kolmas ülesanne

\begin{displaymath}
\resizebox{1.1 \textwidth}{!}
{
\dfrac{
	\dfrac{
		\dfrac{
			\dfrac{
				\dfrac{
					\dfrac{
					}{
						\{x:\alpha, y:\alpha\to\beta\to\gamma, z:\alpha\}\vdash y:\,\alpha\to\beta\to\gamma
					}
				}{
					\{x:\alpha, y:\alpha\to\beta\to\gamma\}\vdash (\lambda z:\alpha. y):\,\alpha\to\alpha\to\beta\to\gamma
				}
				\quad
				\dfrac{
				}{
					\{x:\alpha, y:\alpha\to\beta\to\gamma\}\vdash x:\,\alpha
				}
			}{
				\{x:\alpha, y:\alpha\to\beta\to\gamma\}\vdash  (\lambda z:\alpha. y)\,x :\, \alpha\to\beta\to\gamma
			}
			\quad
			\dfrac{
			}{
				\{x:\alpha, y:\alpha\to\beta\to\gamma\}\vdash  x :\, \alpha
			}
		}{
			\{x:\alpha, y:\alpha\to\beta\to\gamma\}\vdash  (\lambda z:\alpha. y)\,x\,x :\, \beta\to\gamma
		}
	}{
		\{x:\alpha\}\vdash (\lambda y:\alpha\to\beta\to\gamma. (\lambda z:\alpha. y)\,x\,x) :\, \beta\to\gamma
	}
}{
	\vdash (\lambda x:\alpha,\, y:\alpha\to\beta\to\gamma. (\lambda z:\alpha. y)\,x\,x) :\, \beta\to\gamma
}
}
\end{displaymath}

Neljas ülesanne

\begin{displaymath}
\dfrac{
	\dfrac{
		\dfrac{
			\dfrac{
				\dfrac{
					\dfrac{
						\dfrac{
						}{
							G\vdash z:\,\alpha\to(\beta\to\alpha)\to(\beta\to\beta)
						}
						\quad
						\dfrac{
							\dfrac{
							}{
								G\cup\{w:\beta\}\vdash x:\,\alpha
							}
						}{
							G\vdash(\lambda w:\beta. x):\, \beta\to\alpha
						}
					}{
						G\vdash z\,(\lambda w:\beta. x):\, ?
					}
					\quad
					\dfrac{
					}{
						G\vdash y: \beta
					}
				}{
					G\vdash z\,(\lambda w:\beta. x)\,y:\, ?
				}
			}{
				\{x:\alpha, y:\beta, z:\alpha\to(\beta\to\alpha)\to(\beta\to\beta)\}\vdash z\,(\lambda w:\beta. x)\,y :\, ?
			}
		}{
			\{x:\alpha, y:\beta\}\vdash (\lambda z:\alpha\to(\beta\to\alpha)\to(\beta\to\beta). z\,(\lambda w:\beta. x)\,y) :\, ?
		}
	}{
		\{x:\alpha\}\vdash (\lambda y:\beta, z:\alpha\to(\beta\to\alpha)\to(\beta\to\beta). z\,(\lambda w:\beta. x)\,y) :\, ?
	}
}{
	\vdash (\lambda x:\alpha,\, y:\beta, z:\alpha\to(\beta\to\alpha)\to(\beta\to\beta). z\,(\lambda w:\beta. x)\,y) :\, ?
}
\end{displaymath}
Ei saa lahendada, $z$ argumendi tüüp ei klapi $\lambda w:\beta. x$ omaga

\newpage
Viies ülesanne

\begin{displaymath}
\resizebox{1.1 \textwidth}{!}
{
\dfrac{
	\dfrac{
		\dfrac{
			\dfrac{
				\dfrac{
					\dfrac{
					}{
						\{x:\alpha, y:\alpha\to\beta,f:(\alpha\to\beta)\to\alpha\to\beta \}\vdash f:\,(\alpha\to\beta)\to\alpha\to\beta 
					}
				}{
					\{x:\alpha, y:\alpha\to\beta \}\vdash (\lambda f:(\alpha\to\beta)\to\alpha\to\beta. f):\,(\alpha\to\beta)\to\alpha\to\beta 
				}
				\quad
				\dfrac{
				}{
					\{x:\alpha, y:\alpha\to\beta \}\vdash y:\,\alpha\to\beta
				}
			}{
				\{x:\alpha, y:\alpha\to\beta \}\vdash (\lambda f:(\alpha\to\beta)\to\alpha\to\beta. f)\, y:\,\alpha\to\beta
			}
			\quad
			\dfrac{
			}{
				\{x:\alpha, y:\alpha\to\beta \}\vdash x:\,\alpha
			}
		}{
			\{x:\alpha, y:\alpha\to\beta \}\vdash (\lambda f:(\alpha\to\beta)\to\alpha\to\beta. f)\, y\, x\, :\, \beta
		}
	}{
		\{x:\alpha\}\vdash \lambda y:\alpha\to\beta. (\lambda f:(\alpha\to\beta)\to\alpha\to\beta. f)\, y\, x\, :\,\beta
	}
}{
	\vdash \lambda x:\alpha, y:\alpha\to\beta. (\lambda f:(\alpha\to\beta)\to\alpha\to\beta. f)\, y\, x\, :\, \beta
}
}
\end{displaymath}

\end{document}
